\documentclass[letterpaper, 10pt]{article}
\usepackage{amsmath, amsthm, amssymb}
\usepackage{mathtools}
\usepackage{enumitem}
\usepackage{listings}
\usepackage{mathrsfs}

\newtheorem{thm}{Theorem}[section]
\numberwithin{thm}{section}
\newtheorem{axiom}[thm]{Axiom}
\newtheorem{lem}[thm]{Lemma}
\newtheorem{prop}[thm]{Proposition}
\newtheorem{col}[thm]{Corollary}

\theoremstyle{definition}
\newtheorem{mydef}[thm]{Definition}

\setlength\parindent{0pt}

% Def new command for "less than or equal" relation
\newcommand{\ineq}{%
	\mathrel{\mkern1mu\underline{\mkern-1mu\in\mkern-1mu}\mkern1mu}}

\begin{document}

\section{Axioms and Operations}

\begin{axiom}[Extensionality Axiom]
	\begin{equation*}
		\forall A\forall B[\forall x(x \in A \leftrightarrow x \in B)
		\rightarrow A = B]
	\end{equation*}
\end{axiom}

\begin{axiom}[Empty Set Axiom]
	\begin{equation*}
		\exists B \forall x \notin B
	\end{equation*}
\end{axiom}


\begin{axiom}[Pairing Axiom]
	\begin{equation*}
		\forall u \forall v \exists B \forall x(x \in B \leftrightarrow 
		x = u \lor x = v)
	\end{equation*}
\end{axiom}

\begin{axiom}[Power Set Axiom]
	\begin{equation*}
		\forall a \exists B \forall x (x \in B \leftrightarrow x \subseteq a)
	\end{equation*}
\end{axiom}

\begin{enumerate}[label=\arabic*.]
	\item $\forall A \forall x \in A (x \subseteq \bigcup A)$
	\item $A \subseteq B \rightarrow \bigcup A \subseteq \bigcup B$
	\item $\forall x \in \mathscr{A} (x \subseteq B) \rightarrow \bigcup \mathscr{A}
		\subseteq B$
	\item $\bigcup\mathscr{P}A = A$
	\item $A \subseteq \mathscr{P}\bigcup A$
	\item $\mathscr{P}A \cap \mathscr{P}B = \mathscr{P}(A \cap B)$
	\item $\mathscr{P}A \cup \mathscr{P}B \subseteq \mathscr{P}(A \cup B)$
\end{enumerate}

\emph{Commutative laws}
\begin{gather*}
	A \cup B = B \cup A \\
	A \cap B = B \cap A
\end{gather*}

\emph{Associative laws}
\begin{gather*}
	A \cup (B \cup C) = (A \cup B) \cup C \\
	A \cap (B \cap C) = (A \cap B) \cap C
\end{gather*}

\emph{Distributive laws}
\begin{gather*}
	A \cap (B \cup C) = (A \cap B) \cup (A \cap C) \\
	A \cup (B \cap C) = (A \cup B) \cap (A \cup C) \\
	A \cup \bigcap\mathscr{B} = \bigcap \{A \cup X \mid X \in \mathscr{B}\} \\
	A \cap \bigcup\mathscr{B} = \bigcup \{A \cap X \mid X \in \mathscr{B}\}
\end{gather*}

\begin{enumerate}[label=\arabic*.]
	\item $ A \subseteq B \implies C - B \subseteq C - A $
	\item $ x \in A + B \iff x\in (A - B) \cup (B - A) $
	\item $ A \cap (B + C) = (A \cap B) + (A \cap C) $
	\item $ A + (B + C) = (A + B) + C  $
	\item $ A \subseteq B \iff A - B = \emptyset \iff 
		A \cup B = B \iff A \cap B = A  $
	\item $ \bigcup (A \cup B) = \bigcup A \cup \bigcup B $
	\item $ A \ne \emptyset \land B \ne \emptyset \quad \bigcap (A \cup B) =
		\bigcap A \cap \bigcap B $
	\item $ \mathscr{A} \ne \emptyset \quad \mathscr{P}\bigcap\mathscr{A} =
		\bigcap\{\mathscr{P}X \mid X \in \mathscr{A}\} $
	\item $ \bigcup\{\mathscr{P}X \mid X \in \mathscr{A}\} \subseteq 
		\mathscr{P}\bigcup\mathscr{A} $
\end{enumerate}
\end{document}
